Added Reify, Realize and finished basic simplification'

kami_rewrites_reflection.v
@@ -13,24 +13,124 @@ Inductive KRTyp : Type :=
   | KRTypDefMethT: KRTyp
   | KRList: KRTyp -> KRTyp.
 
-Fixpoint KRrealize (t: KRTyp) :=
+Fixpoint KRrealizeType (t: KRTyp) :=
   match t with
   | KRTypModuleElt => ModuleElt
   | KRTypRegInitT => RegInitT
   | KRTypAttributeActionVoid => Attribute (Action Void)
   | KRTypDefMethT => DefMethT
-  | KRList t => list (KRrealize t)
+  | KRList t => list (KRrealizeType t)
   end.
 
-Inductive KRExp : KRTyp -> Type :=
-  | KRVar t : (KRrealize t) -> KRExp t
-  | KRCons t : KRExp t -> KRExp (KRList t) -> KRExp (KRList t)
-  | KRApp t : KRExp (KRList t) -> KRExp (KRList t) -> KRExp (KRList t)
-  | KRMERegister : KRExp KRTypRegInitT -> KRExp KRTypModuleElt
-  | KRRegisters : KRExp (KRList KRTypRegInitT) -> KRExp (KRList KRTypModuleElt)
-  | KRMERule : KRExp KRTypAttributeActionVoid -> KRExp KRTypModuleElt
-  | KRMEMeth : KRExp KRTypDefMethT -> KRExp KRTypModuleElt
-  | KRMakeModule_rules : KRExp (KRList KRTypModuleElt) -> KRExp (KRList KRTypAttributeActionVoid)
-  | KRMakeModule_regs : KRExp (KRList KRTypModuleElt) -> KRExp (KRList KRTypRegInitT)
-  | KRMakeModule_meths : KRExp (KRList KRTypModuleElt) -> KRExp (KRList KRTypDefMethT).
+Inductive KRExp: KRTyp -> Type :=
+  | KRNil t : @KRExp (KRList t)
+  | KRVar t : (KRrealizeType t) -> @KRExp t
+  | KRCons t : @KRExp t -> @KRExp (KRList t) -> @KRExp (KRList t)
+  | KRApp t : @KRExp (KRList t) -> @KRExp (KRList t) -> @KRExp (KRList t)
+  | KRMERegister : @KRExp KRTypRegInitT -> @KRExp KRTypModuleElt
+  | KRRegisters : @KRExp (KRList KRTypRegInitT) -> @KRExp (KRList KRTypModuleElt)
+  | KRMERule : @KRExp KRTypAttributeActionVoid -> @KRExp KRTypModuleElt
+  | KRMEMeth : @KRExp KRTypDefMethT -> @KRExp KRTypModuleElt
+  | KRMakeModule_rules : @KRExp (KRList KRTypModuleElt) -> @KRExp (KRList KRTypAttributeActionVoid)
+  | KRMakeModule_regs : @KRExp (KRList KRTypModuleElt) -> @KRExp (KRList KRTypRegInitT)
+  | KRMakeModule_meths : @KRExp (KRList KRTypModuleElt) -> @KRExp (KRList KRTypDefMethT).
+
+Fixpoint KRRealizeExp {t} (e: KRExp t) :=
+  match e in KRExp t return (KRrealizeType t) with
+  | KRNil t => @nil (@KRrealizeType t)
+  | KRVar t e => e
+  | KRCons t a b => @cons (@KRrealizeType t) (@KRRealizeExp t a) (@KRRealizeExp (KRList t) b)
+  | KRApp t a b => @app (@KRrealizeType t) (@KRRealizeExp (KRList t) a) (@KRRealizeExp (KRList t) b)
+  | KRMERegister e => MERegister (@KRRealizeExp KRTypRegInitT e)
+  | KRRegisters l => Registers (@KRRealizeExp (KRList KRTypRegInitT) l)
+  | KRMERule r => MERule (@KRRealizeExp KRTypAttributeActionVoid r)
+  | KRMEMeth m => MEMeth (@KRRealizeExp KRTypDefMethT m)
+  | KRMakeModule_rules r => makeModule_rules (@KRRealizeExp (KRList KRTypModuleElt) r)
+  | KRMakeModule_regs r => makeModule_regs (@KRRealizeExp (KRList KRTypModuleElt) r)
+  | KRMakeModule_meths m =>makeModule_meths (@KRRealizeExp (KRList KRTypModuleElt) m)
+  end.
+
+Ltac KRReifyExp e t :=
+  match e with
+  | nil => constr:(@KRNil t)
+  | cons ?F ?R => match t with
+                  | KRList ?T => constr:(@KRCons T (ltac:(KRReifyExp F T)) (ltac:(KRReifyExp R t)))
+                  | ?T => constr:(@KRVar t e)
+                  end
+  | app ?F ?R => match t with
+                 | KRList ?T => constr:(@KRApp T (ltac:(KRReifyExp F t)) (ltac:(KRReifyExp R t)))
+                 | ?T => constr:(@KRVar t e)
+                 end
+  | ?X => constr:(@KRVar t X)
+  | MERegister ?E => match t with
+                     | KRTypModuleElt => constr:(@KRMERegister (ltac:(KRReifyExp E KRTypRegInitT)))
+                     | ?T => constr:(@KRVar t e)
+                     end
+  | Registers ?E => match t with
+                    | KRList KRTypModuleElt => constr:(@KRRegisters (ltac:(KRReifyExp E (KRList KRTypRegInitT))))
+                    | ?T => constr:(@KRVar t e)
+                    end
+  | MERule ?E => match t with
+                 | KRTypModuleElt => constr:(@KRMERule (ltac:(KRReifyExp E KRTypAttributeActionVoid)))
+                 | ?T => constr:(@KRVar t e)
+                 end
+  | MEMeth ?E => match t with
+                 | KRTypModuleElt => constr:(@KRMEMeth (ltac:(KRReifyExp E KRTypDefMethT)))
+                 | ?T => constr:(@KRVar t e)
+                 end
+  | makeModule_rules ?E => match t with
+                           | KRList KRTypAttributeActionVoid => constr:(@KRMakeModule_rules (ltac:(KRReifyExp E (KRList KRTypModuleElt))))
+                           | ?T => constr:(@KRVar t e)
+                           end
+  | makeModule_regs ?E => match t with
+                          | KRList KRTypRegInitT => constr:(@KRMakeModule_regs (ltac:(KRReifyExp E (KRList KRTypModuleElt))))
+                          | ?T => constr:(@KRVar t e)
+                          end
+  | makeModule_meths ?E => match t with
+                          | KRList KRTypDefMethT => constr:(@KRMakeModule_meths (ltac:(KRReifyExp E (KRList KRTypModuleElt))))
+                          | ?T => constr:(@KRVar t e)
+                          end
+  end.
+
+Fixpoint KRSimplifyTop {t} (e : KRExp t) :=
+  match e in KRExp t return KRExp t with
+  | @KRApp KRTypModuleElt f c => match f with
+                                 | @KRCons KRTypModuleElt a b => @KRCons KRTypModuleElt a (@KRApp KRTypModuleElt b c)
+                                 | _ => @KRApp KRTypModuleElt f c
+                                 end
+  | KRRegisters x => match x with
+                     | @KRApp KRTypRegInitT a b => @KRApp KRTypModuleElt (KRRegisters a) (KRRegisters b)
+                     | @KRCons KRTypRegInitT a b => @KRCons KRTypModuleElt (KRMERegister a) (KRRegisters b)
+                     | KRNil KRTypModuleElt => KRNil KRTypModuleElt
+                     | e => KRRegisters e
+                     end
+  | e => e
+  end.
+
+Fixpoint KRSimplify {t} (e: KRExp t) :=
+  match e in KRExp t return KRExp t with
+  | @KRCons t a b => KRSimplifyTop (@KRCons t (KRSimplify a) (KRSimplify b))
+  | @KRApp t a b => KRSimplifyTop (@KRApp t (KRSimplify a) (KRSimplify b))
+  | @KRMERegister a => KRSimplifyTop (@KRMERegister (KRSimplify a))
+  | @KRRegisters a => KRSimplifyTop (@KRRegisters (KRSimplify a))
+  | @KRMEMeth a => KRSimplifyTop (@KRMEMeth (KRSimplify a))
+  | @KRMERule a => KRSimplifyTop (@KRMERule (KRSimplify a))
+  | @KRMakeModule_rules a => KRSimplifyTop (@KRMakeModule_rules (KRSimplify a))
+  | @KRMakeModule_regs a => KRSimplifyTop (@KRMakeModule_regs (KRSimplify a))
+  | @KRMakeModule_meths a => KRSimplifyTop (@KRMakeModule_meths (KRSimplify a))
+  | e => e
+  end.
+
+
+Theorem KRSimplifySound: forall t e, @KRRealizeExp t e = @KRRealizeExp t (@KRSimplify t e).
+Admitted.
+
+(*Fixpoint KRSimplifyTop {t} (e : KRExp t) :=
+  match e in KRExp t return KRExp t with
+  (*| KRApp KRTypModuleElt (KRCons KRTypModuleElt a b) c => @KRCons KRTypModuleElt a (@KRApp KRTypModuleElt b c)
+  | KRRegisters (KRCons KRTypRegInitT a b) => @KRCons KRTypModuleElt (KRMERegister a) (KRRegisters b)
+  | KRRegisters (@KRApp KRTypRegInitT a b) => @KRApp KRTypModuleElt (KRRegisters a) (KRRegisters b)*)
+  | @KRRegisters (@KRNil KRTypModuleElt) => @KRNil KRTypModuleElt
+  | e => e
+  end.*)
 
